\begin{problem}{2.5}{problem2_5}
Using the sliding variable $\sigma = x_1$ and the control $u = -\text{sign}(\sigma)$, find the sliding mode equation for the systems given below, by using the equivalent control method and Filippov method for the cases:

\begin{itemize}
	\item[(a)]
		\begin{align*}
			\dot{x}_1 & = u             \\
			\dot{x}_2 & = (2u^2 - 1)x_2
		\end{align*}
	\item[(b)]
		\begin{align*}
			\dot{x}_1 & = u             \\
			\dot{x}_2 & = (u - 2u^3)x_2
		\end{align*}
	\item[(c)]
		\begin{align*}
			\dot{x}_1 & = u             \\
			\dot{x}_2 & = (u - 2u^2)x_2
		\end{align*}
\end{itemize}
\end{problem}

\begin{solution}{}{solution2_5}
	\textbf{(a)}
	\begin{enumerate}
		\item \textbf{Equivalent control Method:}

		      The sliding surface is defined as $\sigma = x_1$. In sliding mode, we require:
		      \begin{align*}
			      \sigma       & = 0, \\
			      \dot{\sigma} & = 0.
		      \end{align*}
		      Since $\dot{\sigma} = \dot{x}_1 = u$, imposing $\dot{\sigma} = 0$ gives:
		      \[
			      u_{eq} = 0.
		      \]

		      Substituting $u_{eq} = 0$ into the second equation:
		      \begin{align*}
			      \dot{x}_2 & = (2(0)^2 - 1)x_2 \\
			                & = -x_2.
		      \end{align*}

		      Thus, the sliding mode dynamics under the equivalent control method are:
		      \[
			      \dot{x}_2 = -x_2.
		      \]
		\item \textbf{Filippov Method:}

		      The actual control law is $u = -\text{sign}(x_1)$, leading to discontinuities at $x_1 = 0$. To apply Filippov's method, we examine the system's behavior on both sides:

		      \begin{itemize}
			      \item If $x_1 > 0$, then $u = -1$.
			      \item If $x_1 < 0$, then $u = +1$.
		      \end{itemize}

		      Substituting into the dynamics:
		      \begin{itemize}
			      \item For $u = -1$:
			            \begin{align*}
				            \dot{x}_1 & = -1,                  \\
				            \dot{x}_2 & = (2(1) - 1)x_2 = x_2.
			            \end{align*}

			      \item For $u = +1$:
			            \begin{align*}
				            \dot{x}_1 & = 1,                   \\
				            \dot{x}_2 & = (2(1) - 1)x_2 = x_2.
			            \end{align*}
		      \end{itemize}

		      The Filippov convex combination requires choosing a mixture such that $\dot{x}_1 = 0$:
		      \[
			      (1-\alpha)(-1) + \alpha(1) = 0 \quad \Rightarrow \quad \alpha = \frac{1}{2}.
		      \]

		      Thus, the sliding dynamics for $x_2$ are:
		      \[
			      \dot{x}_2 = x_2.
		      \]

		\item \textbf{Final Results:}
		      \begin{itemize}
			      \item Equivalent Control Method: $\dot{x}_2 = -x_2$
			      \item Filippov Method: $\dot{x}_2 = x_2$
		      \end{itemize}
	\end{enumerate}
	\textbf{(b)}
	\begin{enumerate}
		\item \textbf{Equivalent control Method:}
		      \[
			      \dot{\sigma} = \dot{x}_1 = u = 0 \Rightarrow u_{eq} = 0.
		      \]
		      Substituting $u_{eq} = 0$:
		      \begin{align*}
			      \dot{x}_1 & = 0, \\
			      \dot{x}_2 & = 0.
		      \end{align*}
		\item \textbf{Filippov Method:}
		      \begin{itemize}
			      \item For $u = -1$:
			            \begin{align*}
				            \dot{x}_1 & = -1, \\
				            \dot{x}_2 & = x_2
			            \end{align*}
			      \item For $u = +1$:
			            \begin{align*}
				            \dot{x}_1 & = 1,   \\
				            \dot{x}_2 & = -x_2
			            \end{align*}
		      \end{itemize}
		      Then, is trivial to see that $\alpha = \frac{1}{2}$ again, so we have:
		      \[
			      \dot{x}_2 = (1-\alpha)(x_2) - \alpha x_2 = 0
		      \]
		\item \textbf{Final Results:}
		      \begin{itemize}
			      \item Equivalent Control Method: $\dot{x}_2 = 0$
			      \item Filippov Method: $\dot{x}_2 = 0$
		      \end{itemize}
	\end{enumerate}
	\textbf{(c)}
	\begin{enumerate}
		\item \textbf{Equivalent control Method:}
		      \[
			      \dot{\sigma} = \dot{x}_1 = u = 0 \Rightarrow u_{eq} = 0.
		      \]
		      Substituting $u_{eq} = 0$:
		      \begin{align*}
			      \dot{x}_1 & = 0, \\
			      \dot{x}_2 & = 0.
		      \end{align*}
		\item \textbf{Filippov Method:}
		      \begin{itemize}
			      \item For $u = -1$:
			            \begin{align*}
				            \dot{x}_1 & = -1,    \\
				            \dot{x}_2 & = -3 x_2
			            \end{align*}
			      \item For $u = +1$:
			            \begin{align*}
				            \dot{x}_1 & = 1,   \\
				            \dot{x}_2 & = -x_2
			            \end{align*}
		      \end{itemize}
		      Then, is trivial to see that $\alpha = \frac{1}{2}$ again, so we have:
		      \[
			      \dot{x}_2 = (1-\alpha)(-3x_2) - \alpha x_2 = -2x_2
		      \]
		\item \textbf{Final Results:}
		      \begin{itemize}
			      \item Equivalent Control Method: $\dot{x}_2 = 0$
			      \item Filippov Method: $\dot{x}_2 = -2x_2$
		      \end{itemize}
	\end{enumerate}


\end{solution}